src/QUIC.Impl.fst
@@ -7,7 +7,7 @@ module IB = LowStar.ImmutableBuffer
 module Seq = QUIC.Secret.Seq
 module HS = FStar.HyperStack
 module ST = FStar.HyperStack.ST
-
+module HST = FStar.HyperStack.ST
 
 module U64 = FStar.UInt64
 module U32 = FStar.UInt32
@@ -37,10 +37,369 @@ open LowStar.BufferOps
 
 #restart-solver
 
+module SAEAD = Spec.Agile.AEAD
+module SCipher = Spec.Agile.Cipher
+
+module SecretBuffer = QUIC.Secret.Buffer
+
+
+(* There are a few places where EverCrypt needs public data whereas it
+could/should be secret. Thus, we may need some declassification
+locally using Lib.RawIntTypes, but we definitely don't want to make
+secret integers globally transparent using friend *)
+
+module ADMITDeclassify = Lib.RawIntTypes
+
+unfold
+let iv_for_encrypt_pre
+  (a: ea)
+  (siv: B.buffer Secret.uint8)
+  (dst: B.buffer Secret.uint8)
+  (h: G.erased Spec.header { ~ (Spec.is_retry h) })
+  (pn_len: PN.packet_number_length_t)
+  (pn: PN.packet_number_t)
+  (m: HS.mem)
+: GTot Type0
+=
+  let a' = SAEAD.cipher_alg_of_supported_alg a in
+  B.all_disjoint [
+    B.loc_buffer siv;
+    B.loc_buffer dst;
+  ] /\
+  B.live m siv /\ B.length siv == 12 /\
+  B.live m dst /\ B.length dst == 12 /\
+  pn_len == Spec.pn_length h /\
+  pn == Spec.packet_number h
+
+unfold
+let iv_for_encrypt_post
+  (a: ea)
+  (siv: B.buffer Secret.uint8)
+  (dst: B.buffer Secret.uint8)
+  (h: G.erased Spec.header { ~ (Spec.is_retry h) })
+  (pn_len: PN.packet_number_length_t)
+  (pn: PN.packet_number_t)
+  (m: HS.mem)
+  (m' : HS.mem)
+: GTot Type0
+=
+  iv_for_encrypt_pre a siv dst h pn_len pn m /\
+  begin
+    B.modifies (B.loc_buffer dst) m m' /\
+    B.as_seq m' dst `Seq.equal`
+      Spec.iv_for_encrypt a (B.as_seq m siv) h
+  end
+
+let iv_for_encrypt
+  (a: ea)
+  (siv: B.buffer Secret.uint8)
+  (dst: B.buffer Secret.uint8)
+  (h: G.erased Spec.header { ~ (Spec.is_retry h) })
+  (pn_len: PN.packet_number_length_t)
+  (pn: PN.packet_number_t)
+: HST.Stack unit
+  (requires (fun m ->
+    iv_for_encrypt_pre a siv dst h pn_len pn m
+  ))
+  (ensures (fun m _ m' ->
+    iv_for_encrypt_post a siv dst h pn_len pn m m'
+  ))
+= let m0 = HST.get () in
+  B.fill dst (Secret.to_u8 0uy) 12ul;
+  let pnb_store = B.sub dst 4ul 8ul in
+  SecretBuffer.store64_be pnb_store pn;
+  let m2 = HST.get () in
+  assert (Seq.seq_reveal (B.as_seq m2 (B.gsub dst 0ul 4ul)) `Seq.equal` Seq.create 4 0uy);
+  assert (Seq.seq_reveal (B.as_seq m2 dst) `Seq.equal` (Seq.create 4 0uy `Seq.append` FStar.Endianness.n_to_be 8 (Secret.v pn)));
+  QUIC.Impl.Lemmas.n_to_be_lower' 8 12 (Secret.v pn);
+  assert (Seq.seq_reveal (B.as_seq m2 dst) == FStar.Endianness.n_to_be 12 (Secret.v pn));
+  QUIC.Impl.Lemmas.op_inplace dst siv 12ul 0ul (Secret.logxor #Secret.U8 #Secret.SEC);
+  QUIC.Impl.Lemmas.secret_xor_inplace_eq (B.as_seq m2 dst) (B.as_seq m2 siv) 0
+
+module SParse = QUIC.Spec.Header.Parse
+
+unfold
+let payload_encrypt_pre
+  (a: ea)
+  (s: AEAD.state a)
+  (siv: B.buffer Secret.uint8)
+  (dst: B.buffer Secret.uint8)
+  (h: G.erased Spec.header { ~ (Spec.is_retry h) })
+  (pn_len: PN.packet_number_length_t)
+  (pn: PN.packet_number_t)
+  (header_len: Secret.uint32)
+  (plain: B.buffer Secret.uint8)
+  (plain_len: Secret.uint32) // should be secret, because otherwise one can compute the packet number length
+  (m: HS.mem)
+: GTot Type0
+=
+  let fmt = SParse.format_header h in
+
+  B.all_disjoint [
+    AEAD.footprint m s;
+    B.loc_buffer siv;
+    B.loc_buffer dst;
+    B.loc_buffer plain;
+  ] /\
+
+  AEAD.invariant m s /\
+  B.live m siv /\ B.length siv == 12 /\
+  Secret.v header_len == Seq.length fmt /\
+  B.live m dst /\ B.length dst == Secret.v header_len + Secret.v plain_len + SAEAD.tag_length a /\
+  pn_len == Spec.pn_length h /\
+  pn == Spec.packet_number h /\
+  B.live m plain /\ B.length plain == Secret.v plain_len /\ 3 <= Secret.v plain_len /\ Secret.v plain_len < max_plain_length /\
+  B.as_seq m (B.gsub dst 0ul (Secret.reveal header_len)) `Seq.equal` Seq.seq_hide fmt
+
+unfold
+let payload_encrypt_post
+  (a: ea)
+  (s: AEAD.state a)
+  (siv: B.buffer Secret.uint8)
+  (dst: B.buffer Secret.uint8)
+  (h: G.erased Spec.header { ~ (Spec.is_retry h) })
+  (pn_len: PN.packet_number_length_t)
+  (pn: PN.packet_number_t)
+  (header_len: Secret.uint32)
+  (plain: B.buffer Secret.uint8)
+  (plain_len: Secret.uint32)
+  (m: HS.mem)
+  (res: error_code)
+  (m' : HS.mem)
+: GTot Type0
+=
+  let fmt = SParse.format_header h in
+  payload_encrypt_pre a s siv dst h pn_len pn header_len plain plain_len m /\
+  B.modifies (B.loc_buffer (B.gsub dst (Secret.reveal header_len) (B.len dst ` U32.sub` Secret.reveal header_len)) `B.loc_union` AEAD.footprint m s) m m' /\
+  AEAD.invariant m' s /\ AEAD.footprint m' s == AEAD.footprint m s /\
+  AEAD.preserves_freeable s m m' /\
+  AEAD.as_kv (B.deref m' s) == AEAD.as_kv (B.deref m s) /\
+  B.as_seq m' (B.gsub dst (Secret.reveal header_len) (B.len dst `U32.sub` Secret.reveal header_len)) `Seq.equal` Seq.seq_hide (Spec.payload_encrypt a (AEAD.as_kv (B.deref m s)) (B.as_seq m siv) h (Seq.seq_reveal (B.as_seq m plain))) /\
+  res == Success
+
+#push-options "--z3rlimit 32"
+
+let payload_encrypt
+  (a: ea)
+  (s: AEAD.state a)
+  (siv: B.buffer Secret.uint8)
+  (dst: B.buffer Secret.uint8)
+  (h: G.erased Spec.header { ~ (Spec.is_retry h) })
+  (pn_len: PN.packet_number_length_t)
+  (pn: PN.packet_number_t)
+  (header_len: Secret.uint32)
+  (plain: B.buffer Secret.uint8)
+  (plain_len: Secret.uint32)
+: HST.Stack error_code
+  (requires (fun m ->
+    payload_encrypt_pre a s siv dst h pn_len pn header_len plain plain_len m
+  ))
+  (ensures (fun m res m' ->
+    payload_encrypt_post a s siv dst h pn_len pn header_len plain plain_len m res m'
+  ))
+= 
+  let m0 = HST.get () in
+  HST.push_frame ();
+  let m1 = HST.get () in
+  B.loc_unused_in_not_unused_in_disjoint m1;
+  let iv = B.alloca (Secret.to_u8 0uy) 12ul in
+
+  (* EverCrypt currently does not support secret length encryption, so
+  whenever we need to define the arguments to EverCrypt.AEAD.encrypt,
+  we need to (locally there and only there) declassify the lengths of
+  the aad, plain, cipher and tag buffers. *)
+  let aad = B.sub dst 0ul (ADMITDeclassify.u32_to_UInt32 header_len) in
+  let cipher = B.sub dst (ADMITDeclassify.u32_to_UInt32 header_len) (ADMITDeclassify.u32_to_UInt32 plain_len) in
+  let tag = B.sub dst (ADMITDeclassify.u32_to_UInt32 (header_len `Secret.add` plain_len)) 16ul in
+
+  iv_for_encrypt a siv iv h pn_len pn;
+  let res = AEAD.encrypt #a s iv 12ul aad (ADMITDeclassify.u32_to_UInt32 header_len) plain (ADMITDeclassify.u32_to_UInt32 plain_len) cipher tag in
+  HST.pop_frame ();
+  res
+
+#pop-options
+
+unfold
+let encrypt'_pre
+  (a: ea)
+  (aead: AEAD.state a)
+  (siv: B.buffer Secret.uint8)
+  (ctr: CTR.state (SAEAD.cipher_alg_of_supported_alg a))
+  (hpk: B.buffer Secret.uint8)
+  (dst: B.buffer U8.t)
+  (h: header)
+  (pn: PN.packet_number_t)
+  (plain: B.buffer Secret.uint8)
+  (plain_len: Secret.uint32) // should be secret, because otherwise one can compute the packet number length
+  (m: HS.mem)
+: GTot Type0
+=
+  let a' = SAEAD.cipher_alg_of_supported_alg a in
+  B.all_disjoint [
+    AEAD.footprint m aead;
+    B.loc_buffer siv;
+    CTR.footprint m ctr;
+    B.loc_buffer hpk;
+    B.loc_buffer dst;
+    header_footprint h;
+    B.loc_buffer plain;
+  ] /\
+  AEAD.invariant m aead /\
+  B.live m siv /\ B.length siv == 12 /\
+  CTR.invariant m ctr /\
+  B.live m hpk /\ B.length hpk == Spec.Agile.Cipher.key_length a' /\
+  B.live m dst /\
+  header_live h m /\
+  B.live m plain /\ B.length plain == Secret.v plain_len /\
+  begin
+    if is_retry h
+    then
+      B.length plain == 0 /\
+      B.length dst == Secret.v (header_len h)
+    else
+      B.length dst == Secret.v (header_len h) + Secret.v plain_len + SAEAD.tag_length a /\
+      3 <= Secret.v plain_len /\ Secret.v plain_len < max_plain_length
+  end
+
+unfold
+let encrypt'_post
+  (a: ea)
+  (aead: AEAD.state a)
+  (siv: B.buffer Secret.uint8)
+  (ctr: CTR.state (SAEAD.cipher_alg_of_supported_alg a))
+  (hpk: B.buffer Secret.uint8)
+  (dst: B.buffer U8.t)
+  (h: header)
+  (pn: PN.packet_number_t)
+  (plain: B.buffer Secret.uint8)
+  (plain_len: Secret.uint32)
+  (m: HS.mem)
+  (res: error_code)
+  (m' : HS.mem)
+: GTot Type0
+=
+  encrypt'_pre a aead siv ctr hpk dst h pn plain plain_len m /\
+  B.modifies (B.loc_buffer dst `B.loc_union` AEAD.footprint m aead `B.loc_union` CTR.footprint m ctr) m m' /\
+  AEAD.invariant m' aead /\ AEAD.footprint m' aead == AEAD.footprint m aead /\
+  AEAD.preserves_freeable aead m m' /\
+  AEAD.as_kv (B.deref m' aead) == AEAD.as_kv (B.deref m aead) /\
+  CTR.invariant m' ctr /\ CTR.footprint m' ctr == CTR.footprint m ctr /\
+  B.as_seq m' dst `Seq.equal` Spec.encrypt a (AEAD.as_kv (B.deref m aead)) (B.as_seq m siv) (B.as_seq m hpk) (g_header h m pn) (Seq.seq_reveal (B.as_seq m plain)) /\
+  res == Success
+
+#push-options "--z3rlimit 64"
+
+let encrypt'
+  (a: ea)
+  (aead: AEAD.state a)
+  (siv: B.buffer Secret.uint8)
+  (ctr: CTR.state (SAEAD.cipher_alg_of_supported_alg a))
+  (hpk: B.buffer Secret.uint8)
+  (dst: B.buffer U8.t)
+  (h: header)
+  (pn: PN.packet_number_t)
+  (plain: B.buffer Secret.uint8)
+  (plain_len: Secret.uint32)
+: HST.Stack error_code
+  (requires (fun m ->
+    encrypt'_pre a aead siv ctr hpk dst h pn plain plain_len m
+  ))
+  (ensures (fun m res m' ->
+    encrypt'_post a aead siv ctr hpk dst h pn plain plain_len m res m'
+  ))
+= let m0 = HST.get () in
+  let gh = Ghost.hide (g_header h m0 pn) in
+  let fmt = Ghost.hide (QUIC.Spec.Header.Parse.format_header gh) in
+  let header_len = header_len h in
+  QUIC.Impl.Header.Parse.header_len_correct h m0 pn;
+  QUIC.Impl.Header.Base.header_len_v h;
+  let is_retry = is_retry h in
+
+  (* Currently, EverParse needs the size of the destination buffer for
+  writing, as a public integer, even though this is not strictly
+  necessary. Since the serializers have no knowledge of the payload,
+  and do not perform any declassification of the header sizes, we can
+  pass the whole size of the destination buffer. *)
+  QUIC.Impl.Header.Parse.write_header h pn dst
+    (ADMITDeclassify.u32_to_UInt32 (header_len `Secret.add` (if is_retry then Secret.to_u32 0ul else plain_len `Secret.add` Secret.to_u32 16ul)));
+
+  if is_retry
+  then begin
+    Success
+  end
+  else begin
+    let m1 = HST.get () in
+    let pn_len = pn_length h in
+    let res = SecretBuffer.with_whole_buffer_hide_weak_modifies
+      #error_code
+      dst
+      m1
+      (AEAD.footprint m0 aead `B.loc_union`
+        B.loc_buffer siv `B.loc_union`
+        CTR.footprint m0 ctr `B.loc_union`
+        B.loc_buffer hpk `B.loc_union`
+        B.loc_buffer plain)
+      (AEAD.footprint m0 aead)
+      true
+      (fun res cont m_ ->
+        res == Success /\
+        cont `Seq.equal` (
+          fmt `Seq.append`
+          Spec.payload_encrypt a (AEAD.as_kv (B.deref m0 aead)) (B.as_seq m0 siv) (g_header h m0 pn) (Seq.seq_reveal (B.as_seq m0 plain))) /\
+        AEAD.invariant m_ aead /\ AEAD.footprint m_ aead == AEAD.footprint m0 aead /\
+        AEAD.preserves_freeable aead m1 m_ /\
+        AEAD.as_kv (B.deref m_ aead) == AEAD.as_kv (B.deref m0 aead)
+      )
+      (fun _ bs -> 
+        let res = payload_encrypt a aead siv bs gh pn_len pn header_len plain plain_len in
+        let m_ = HST.get () in
+        assert (
+          let cont = B.as_seq m_ bs in
+          Seq.length fmt == Secret.v header_len /\
+          cont `Seq.equal` (Seq.slice cont 0 (Secret.v header_len) `Seq.append` Seq.slice cont (Secret.v header_len) (Seq.length cont))
+        );
+        res
+      )
+    in
+    match res with
+    | Success ->
+      let m3 = HST.get () in
+      assert (
+        Seq.slice (B.as_seq m3 dst) (Secret.v header_len) (B.length dst) `Seq.equal` Spec.payload_encrypt a (AEAD.as_kv (B.deref m0 aead)) (B.as_seq m0 siv) gh (Seq.seq_reveal (B.as_seq m0 plain))
+      );
+      QUIC.Impl.Header.header_encrypt a ctr hpk dst gh (BShort? h) is_retry (public_header_len h) pn_len;
+      let m4 = HST.get () in
+      assert (B.as_seq m4 dst `Seq.equal` QUIC.Spec.Header.header_encrypt a (B.as_seq m0 hpk) gh (Spec.payload_encrypt a (AEAD.as_kv (B.deref m0 aead)) (B.as_seq m0 siv) gh (Seq.seq_reveal (B.as_seq m0 plain))));
+      res
+    | _ ->
+      assert False;
+      res
+  end
+
+#pop-options
+
+(* At this point I need to have access to the internal state *)
+friend QUIC.Impl.Crypto
+
+#push-options "--z3rlimit 64"
+
 let encrypt
   #i s dst dst_pn h plain plain_len
-= assume False;
-  UnsupportedAlgorithm
+=
+  let m0 = HST.get () in
+  let QUIC.Impl.Crypto.State hash_alg aead_alg e_traffic_secret e_initial_pn
+    aead_state iv hp_key bpn ctr_state = !*s
+  in
+  let last_pn = !* bpn in
+  let pn = last_pn `Secret.add` Secret.to_u64 1uL in
+  B.upd bpn 0ul pn;
+  B.upd dst_pn 0ul pn;
+  let m1 = HST.get () in
+  assert (B.modifies (footprint m0 s `B.loc_union` B.loc_buffer dst_pn) m0 m1);
+  frame_header h pn  (footprint m0 s `B.loc_union` B.loc_buffer dst_pn) m0 m1;
+  encrypt' aead_alg aead_state iv ctr_state hp_key dst h pn plain (Secret.to_u32 plain_len)
+
+#pop-options
 
 (*
 #push-options "--z3rlimit 256"
@@ -289,13 +648,6 @@ let header_encrypt i dst dst_len s h cipher pn =
   end
 
 #pop-options
-
-let tag_len (a: QUIC.Spec.ea): x:U32.t { U32.v x = Spec.Agile.AEAD.tag_length a /\ U32.v x = 16} =
-  let open Spec.Agile.AEAD in
-  match a with
-  | CHACHA20_POLY1305 -> 16ul
-  | AES128_GCM        -> 16ul
-  | AES256_GCM        -> 16ul
 
 (*
 inline_for_extraction
