src/QUIC.Impl.Header.Base.fst
@@ -260,3 +260,11 @@ let header_len_not_is_retry
 = ()
 
 #pop-options
+
+let header_len_v
+  (h: header)
+: Lemma
+  (Secret.v (header_len h) == U32.v (public_header_len h) + (if is_retry h then 0 else Secret.v (pn_length h)))
+= if is_retry h
+  then header_len_is_retry h
+  else header_len_not_is_retry h
